Added more tests for non-deterministic behavior

test/case-studies/sum-to-n.bpl
@@ -3,15 +3,14 @@ procedure main() returns () {
     var sumTo: int;
     var sum: int; 
     var iter: int;
-    sumTo:=101;
+    sumTo:=100;
     sum:=0;
-    iter:=1;
+    iter:=0;
 
-    while (iter != sumTo) invariant sum * 2 == (iter * (iter - 1)); {
-        sum := sum + iter; 
+    while (iter != sumTo) invariant sum * 2 == iter * (iter + 1); {
         iter := iter + 1;
+        sum := sum + iter; 
     }
 
     assert sum == 5050;
 }
-
