test/case-studies/coin-flip.bpl
@@ -1,0 +1,22 @@
+
+procedure main() returns () {
+    var numFlips: int;
+    var iter: int;
+    var heads: int; 
+    var tails: int;
+    numFlips:=100;
+    iter:=0;
+    heads:=0;
+    tails:=0;
+
+    while (iter != numFlips) invariant heads + tails == iter; {
+        iter := iter + 1;
+        if (*) {
+            heads := heads + 1;
+        } else {
+            tails := tails + 1;
+        }
+    }
+
+    assert heads + tails == numFlips;
+}
