test/havoc/max.bpl
@@ -1,0 +1,18 @@
+
+procedure main() returns () {
+    var in1: int;
+    var in2: int;
+    var max: int;
+
+    havoc in1;
+    havoc in2;
+
+    if (in1 > in2) {
+        max := in1;
+    } else {
+        max := in2;
+    }
+
+    assert max >= in1;
+    assert max >= in2;
+}
