test/havoc/square-input.bpl
@@ -1,0 +1,11 @@
+
+procedure main() returns () {
+    var input: int;
+    var squared: int;
+
+    havoc input; 
+    squared := input * input;
+
+    assert squared >= input;
+    assert squared >= 0;
+}
